some fixes

Helpers/Structs.dfy
@@ -35,46 +35,38 @@ module Structs {
   }
 
     class SSL_CTX {
-        var cert_chain : array<string>;
-        var X509 : string;
-        var reference_count : int;
+        var cert_store : array<X509?>;
+        var references : int;
         var meth : string; // method
-        var min_proto_version : int;
-        var max_proto_version : int;
-        var mode : int; //should be unsigned but idk if that matters
-        var session_cache_mode : string;
-        var session_cache_size : int;
 
         method Init()
             // modifies this
             // ensure that all fields have been set
         {
-            // FIXME - change these later
-            X509 := "";
-            cert_chain := new string[maxSize];
+            cert_store := new X509?[maxSize];
 
-            // this is what SSl_CTX_new sets when it is called, resources are freed when this is 0
-            reference_count := 1;
+            //resources are freed when this is 0
+            references := 1;
         }
 
         predicate Valid()
             reads this
         {
-            reference_count != 0
+            references != 0
             // FIXME - this predicate is unfinished
         }
     }
 
+    class X509 {
+
+    }
+
     class tls_opts {
         var tls_ctx : SSL_CTX?;
-        var next : tls_opts?;
-
-        // FIXME - not sure if we need the following fields yet
         // char *app_path
         // int custom_validation
         // int is_server
         // char alpn_string[ALPN_STRING_MAXLEN]
-        // struct tls_opts* next
 
         method Init()
             modifies this
@@ -83,6 +75,10 @@ module Structs {
             tls_ctx := new SSL_CTX;
             tls_ctx.Init();
         }
+    }
+
+    class tls_opts_seq {
+      var opts_list : seq<tls_opts?>;
     }
 
     class tls_conn_ctx {
