tls_wrapper.dfy
@@ -24,13 +24,13 @@ module tls_wrapper {
         }
     }
 
-    method set_certificate_chain(tls_opts : tls_opts, conn_ctx : tls_conn_ctx, filepath : string) returns (y : int)
-        requires tls_opts != null
+    method set_certificate_chain(tls_opts_seq : tls_opts_seq, conn_ctx : tls_conn_ctx, filepath : string) returns (y : int)
+        requires tls_opts_seq != null
         // requires filepath != null
         // ensures that there is a valid cetificate chain set afterward
         ensures y != 0
       {
-        var cur_opts := new tls_opts;
+        var cur_opts := new tls_opts_seq;
         var new_opts := new tls_opts;
 
         // if a connection already exists, set the certs on the existing connection
@@ -41,7 +41,7 @@ module tls_wrapper {
             // SSL_use_certificate_chain_file here loads 
             // contents of filepath into conn_ctx.tls
             conn_ctx.tls := filepath;
-            assert conn_ctx.tls != null; // FIXME
+            assert conn_ctx.tls != null;
           }
           else {
             // compat_SSL_use_certificate_chain_file here 
@@ -55,11 +55,12 @@ module tls_wrapper {
         }
 
         // if no connection exists, set the certs on the options
-        if tls_opts == null {
+        if tls_opts_seq == null {
           return 0;
         }
 
-        cur_opts := tls_opts;
+
+        cur_opts := tls_opts_seq.opts_list[0];
         // There is no cert set yet on the first SSL_CTX so we'll use that
         if (SSL_CTX_get0_certificate(cur_opts.tls_ctx) == "") { // called from OpenSSLHelpers
         	if (SSL_CTX_use_certificate_chain_file(cur_opts.tls_ctx, filepath) != 1) {
@@ -68,10 +69,7 @@ module tls_wrapper {
         	return 1; //Log: Using cert located at "filepath"
         }
 
-        // Otherwise create a new options struct and use that
-        while (cur_opts.next != NULL) {
-        	cur_opts := cur_opts.next;
-        }
+        cur_opts := tls_opts_seq.opts_list[|tls_opts_seq.opts_list| - 1];
 
         new_opts := tls_opts_create(NULL);
         if (new_opts == NULL) {
@@ -82,7 +80,7 @@ module tls_wrapper {
         	return 0; //Error: Unable to assign certificate chain
         }
         // Add new opts to option list
-        cur_opts.next := new_opts;
+        tls_opts_seq.opts_list := tls_opts_seq.opts_list + [new_opts];
         return 1; //Log: Using cert located at "filepath"
       }
 
